theories/LogicalRelation/Reflexivity.v
@@ -1,5 +1,6 @@
 From LogRel.AutoSubst Require Import core unscoped Ast.
-From LogRel Require Import Utils BasicAst Notations Context Untyped Weakening GenericTyping LogicalRelation Reduction LRInduction Escape.
+From LogRel Require Import Utils BasicAst Notations Context Untyped Weakening GenericTyping LogicalRelation Reduction.
+From LogRel.LogicalRelation Require Import Induction Escape.
 
 Set Universe Polymorphism.
 
