theories/LogicalRelation/ShapeView.v
@@ -1,5 +1,6 @@
 From LogRel.AutoSubst Require Import core unscoped Ast.
-From LogRel Require Import Utils BasicAst Notations Context Untyped UntypedReduction GenericTyping LogicalRelation Reduction LRInduction Reflexivity.
+From LogRel Require Import Utils BasicAst Notations Context Untyped UntypedReduction GenericTyping LogicalRelation Reduction.
+From LogRel.LogicalRelation Require Import Induction Reflexivity.
 
 Set Universe Polymorphism.
 
