theories/LogicalRelation/Weakening.v
@@ -1,0 +1,135 @@
+From LogRel.AutoSubst Require Import core unscoped Ast.
+From LogRel Require Import Utils BasicAst Notations Context Untyped Weakening GenericTyping LogicalRelation Reduction.
+From LogRel.LogicalRelation Require Import Induction Irrelevance.
+
+Set Universe Polymorphism.
+
+Ltac bsimpl' := repeat (first
+                 [ progress setoid_rewrite substSubst_term_pointwise
+                 | progress setoid_rewrite substSubst_term
+                 | progress setoid_rewrite substRen_term_pointwise
+                 | progress setoid_rewrite substRen_term
+                 | progress setoid_rewrite renSubst_term_pointwise
+                 | progress setoid_rewrite renSubst_term
+                 | progress setoid_rewrite renRen'_term_pointwise
+                 | progress setoid_rewrite renRen_term
+                 | progress setoid_rewrite varLRen'_term_pointwise
+                 | progress setoid_rewrite varLRen'_term
+                 | progress setoid_rewrite varL'_term_pointwise
+                 | progress setoid_rewrite varL'_term
+                 | progress setoid_rewrite rinstId'_term_pointwise
+                 | progress setoid_rewrite rinstId'_term
+                 | progress setoid_rewrite instId'_term_pointwise
+                 | progress setoid_rewrite instId'_term
+                 | progress setoid_rewrite wk_to_ren_id
+                 | progress setoid_rewrite wk_compose_compose
+                 | progress setoid_rewrite id_ren
+                 | progress unfold up_term_term, upRen_term_term, up_ren, wk_well_wk_compose, wk_id, wk_step, wk_up, wk_empty (**, _wk_up, _wk_step *)
+                 | progress cbn[subst_term ren_term wk wk_to_ren]
+                 | progress fsimpl ]).
+
+Ltac bsimpl := check_no_evars;
+                repeat
+                 unfold VarInstance_term, Var, ids, Ren_term, Ren1, ren1,
+                  Up_term_term, Up_term, up_term, Subst_term, Subst1, subst1,
+                  RenWk_term, RenWk_subst, RenWlWk_term, RenWlWk_subst
+                  in *; bsimpl'; minimize.
+
+Ltac irrelevance0 :=
+  lazymatch goal with
+  | [|- [_ | _ ||- _ ≅ _ ] ] => eapply LRTyEqIrrelevant'
+  | [|- [_ ||-<_> _ ≅ _ | _ ] ] => eapply LRTyEqIrrelevant'
+  | [|- [_ | _ ||- _ : _ ] ] => eapply LRTmRedIrrelevant'
+  | [|- [_ ||-<_> _ : _ | _ ] ] => eapply LRTmRedIrrelevant'
+  | [|- [_ | _ ||- _ ≅ _ : _ | _ ] ] => eapply LRTmEqIrrelevant'
+  | [|- [_ ||-<_> _ ≅ _ : _ | _ ] ] => eapply LRTmEqIrrelevant'
+  end.
+  
+Ltac irrelevance := irrelevance0 ; [|eassumption] ; try first [reflexivity| now bsimpl].
+
+
+Section Weakenings.
+  Context `{GenericTypingProperties}.
+
+
+  Lemma wkΠ  {Γ Δ A l} (ρ : Δ ≤ Γ) (wfΔ : [|- Δ]) (ΠA : [Γ ||-Π< l > A])
+    (ihdom : forall Δ' (ρ' : Δ' ≤ Δ), [ |- Δ'] -> [Δ' ||-< l > ⟨ρ'⟩ (⟨ρ⟩ (PiRedTyPack.dom ΠA))])
+    (ihcod : forall (a : term), [PiRedTyPack.domRed ΠA ρ wfΔ | _ ||- a : _] ->
+      forall Δ' (ρ' : Δ' ≤ Δ), [ |- Δ'] ->
+      [Δ' ||-< l > ⟨ρ'⟩ (PiRedTyPack.cod ΠA)[a .: ρ >> tRel]]) :
+    [Δ ||-Π< l > ⟨ρ⟩ A].
+  Proof.
+    destruct ΠA as[na dom cod];  cbn -[RenWlWk_term] in *.
+    assert (domRed' : forall Δ' (ρ' : Δ' ≤ Δ), [|- Δ'] -> [Δ' ||-< l > ⟨ρ'⟩ (⟨ρ⟩ dom)]).
+    {
+      intros ? ρ' ?; replace (⟨ _ ⟩ _) with (⟨ρ' ∘w ρ⟩ dom) by now bsimpl.
+      econstructor; now unshelve eapply domRed.
+    }
+    set (cod' := ⟨wk_up na dom ρ⟩cod).
+    assert (codRed' : forall Δ' a (ρ' : Δ' ≤ Δ) (h : [|- Δ']),
+      [domRed' Δ' ρ' h | _ ||- a : _] -> [Δ' ||-< l > cod'[a .: ρ' >> tRel]]).
+    {
+      intros ? a ρ' ?.
+      replace (cod'[a .: ρ' >> tRel]) with (cod[ a .: (ρ' ∘w ρ) >> tRel]) by (unfold cod'; now bsimpl).
+      econstructor; unshelve eapply codRed; [assumption|].
+      irrelevance.
+    }
+    exists na (dom ⟨ρ⟩) cod' domRed' codRed'.
+    + unfold cod'; change (tProd ?na _ _) with ((tProd na dom cod)⟨ρ⟩);  gen_typing.
+    + gen_typing.
+    + unfold cod'; set (ρ1 := wk_up na (dom) ρ); eapply wft_wk; gen_typing.
+    + unfold cod'; change (tProd ?na _ _) with ((tProd na dom cod)⟨ρ⟩);  gen_typing.
+    + intros Δ' a b ρ' wfΔ' ???. 
+      replace (cod'[b .: ρ' >> tRel]) with (cod[ b .: (ρ' ∘w ρ) >> tRel]) by (unfold cod'; now bsimpl).
+      subst cod'; unshelve epose (codExt Δ' a b (ρ' ∘w ρ) wfΔ' _ _ _); irrelevance.
+  Defined.
+
+
+  Lemma wk {Γ Δ A l} (ρ : Δ ≤ Γ) (wfΔ : [|- Δ]) :
+    [Γ ||-<l> A] -> [Δ ||-<l> A⟨ρ⟩].
+  Proof.
+    intros lrA. revert Δ ρ wfΔ . pattern l, Γ, A, lrA.
+    eapply LR_rect_TyUr; clear l Γ A lrA.
+    - intros **. cbn. apply LRU_. now econstructor.
+    - intros ???[ty]???. apply LRne_. 
+      exists (⟨ρ⟩ ty); [|now apply whne_ren|change U with U⟨ρ⟩] ;gen_typing.
+    - intros ??? ? ihdom ihcod ???. apply LRPi'; eapply (wkΠ ρ wfΔ ΠA).
+      + intros; apply ihdom; assumption.
+      + intros; eapply ihcod; eassumption.
+  Defined.
+
+  Lemma wkΠ_eq {Γ Δ A l} (ρ : Δ ≤ Γ) (wfΔ : [|- Δ]) (ΠA : [Γ ||-Π< l > A]) :
+    let ihdom Δ' (ρ' : Δ' ≤ Δ) (h : [ |- Δ']) := wk ρ' h (PiRedTyPack.domRed ΠA ρ wfΔ) in
+    let ihcod a (ha : [PiRedTyPack.domRed ΠA ρ wfΔ | _ ||- a : _]) Δ' (ρ' : Δ' ≤ Δ) (h : [ |- Δ']) :=
+      wk ρ' h (PiRedTyPack.codRed ΠA ρ wfΔ ha) 
+    in
+    wk ρ wfΔ (LRPi' l ΠA) = LRPi' l (wkΠ ρ wfΔ ΠA ihdom ihcod).
+  Proof. reflexivity. Qed.
+
+  Set Printing Primitive Projection Parameters.
+
+  Lemma wkEq {Γ Δ A B l} (ρ : Δ ≤ Γ) (wfΔ : [|-Δ]) (lrA : [Γ ||-<l> A]) : 
+    [Γ ||-<l> A ≅ B | lrA] -> [Δ ||-<l> A⟨ρ⟩ ≅ B⟨ρ⟩ | wk ρ wfΔ lrA].
+  Proof.
+    revert B Δ ρ wfΔ. pattern l, Γ, A, lrA.
+    eapply LR_rect_TyUr; clear l Γ A lrA.
+    - intros ? ????? [->]; now constructor.
+    - intros * [ty]. exists ty⟨ρ⟩.
+      1,2: gen_typing. 
+      cbn -[RenWlWk_term]; change U with U⟨ρ⟩; eapply convneu_wk; assumption.
+    - intros * ihdom ihcod * [na dom cod]. rewrite wkΠ_eq. set (X := wkΠ _ _ _ _ _).
+      exists na (dom⟨ρ⟩) (cod⟨wk_up na dom ρ⟩). cbn -[RenWlWk_term] in *.
+      + abstract (change (tProd ?na _ _) with ((tProd na dom cod)⟨ρ⟩);  gen_typing).
+      + change (tProd na _ _) with ((tProd na dom cod)⟨ρ⟩).
+        replace (tProd _ _ _) with ((PiRedTyPack.prod _ ΠA)⟨ρ⟩) by now bsimpl.
+        eapply convty_wk; assumption.
+      + intros. unshelve eapply LRTyEqIrrelevant.
+        3: unshelve eapply ihdom; try eassumption; eapply domRed.
+      + intros ? a ρ' ??.
+        replace (_[_ .: ρ' >> tRel]) with (cod[ a .: (ρ' ∘w ρ) >> tRel]) by now bsimpl.
+        irrelevance0.
+        2: unshelve eapply codRed; [eassumption|]; subst X; irrelevance.
+        subst X; bsimpl; rewrite scons_comp'; reflexivity.
+  Qed.
+
+End Weakenings.
