theories/Substitution/Properties.v
@@ -1,5 +1,6 @@
 From LogRel.AutoSubst Require Import core unscoped Ast.
-From LogRel Require Import Utils BasicAst Notations Context Untyped Weakening GenericTyping LogicalRelation Reduction Irrelevance Escape Reflexivity Validity.
+From LogRel Require Import Utils BasicAst Notations Context Untyped Weakening GenericTyping LogicalRelation Reduction Validity.
+From LogRel.LogicalRelation Require Import Irrelevance Escape Reflexivity.
 From LogRel.Substitution Require Import Irrelevance.
 
 Section Properties.
